platform/cito/GetLocalVarsFacts.v
@@ -1,14 +1,8 @@
 Set Implicit Arguments.
 
-Require Import Equalities.
 Require Import StringSet.
-Module Import SS := StringSet.
-Require Import SetFacts.
-Require Import FSetFacts1.
-Module SK_as_UDT := Make_UDT StringKey.
-Require Import FSetFacts1.
-Module Import SF1 := UWFacts_fun SK_as_UDT SS.
-Import P FM.
+Import StringSet.
+Require Import StringSetFacts.
 
 Section TopSection.
 
@@ -18,7 +12,7 @@ Section TopSection.
   Lemma get_local_vars_cardinal : forall s1 s2 argvars retvar, Subset (free_vars s1) (free_vars s2) -> length (get_local_vars s1 argvars retvar) <= length (get_local_vars s2 argvars retvar).
     intros.
     unfold get_local_vars.
-    repeat rewrite <- SS.cardinal_1.
+    repeat rewrite <- StringSet.cardinal_1.
     eapply subset_cardinal.
     eapply diff_s_m.
     eapply add_s_m; eauto.
@@ -38,7 +32,7 @@ Section TopSection.
     destruct (List.In_dec string_dec a argvars).
     eapply in_or_app; eauto.
     eapply in_or_app; right.
-    eapply InA_eq_List_In.
+    eapply InA_eq_In_iff.
     eapply elements_iff.
     eapply diff_iff.
     split.
