platform/cito/PostOk.v
@@ -57,7 +57,7 @@ Module Make (Import E : ADT) (Import M : RepInv E).
       Require Import ListFactsNew.
       Require Import StringSet.
       Import StringSet.
-      Require Import SetFacts.
+      Require Import StringSetTactics.
       Require Import GeneralTactics.
       Require Import WordFacts.
       Require Import SynReqFacts2.
